Clase5.Listas.fst
@@ -11,12 +11,19 @@ let rec sum_int xs =
 (* Demuestre que sum_int "distribuye" sobre la concatenación de listas. *)
 let rec sum_append (l1 l2 : list int)
   : Lemma (sum_int (l1 @ l2) == sum_int l1 + sum_int l2)
-  = admit()
+  = 
+    match l1 with
+    | [] -> ()
+    | _::xs -> sum_append xs l2
+
 
 (* Idem para length, definida en la librería de F*. *)
 let rec len_append (l1 l2 : list int)
   : Lemma (length (l1 @ l2) == length l1 + length l2)
-  = admit()
+  =
+    match l1 with
+    | [] -> ()
+    | _::xs -> len_append xs l2
 
 let rec snoc (xs : list int) (x : int) : list int =
   match xs with
@@ -32,14 +39,54 @@ let rec rev_int (xs : list int) : list int =
   | [] -> []
   | x::xs' -> snoc (rev_int xs') x
 
-let rev_append_int (xs ys : list int)
-  : Lemma (rev_int (xs @ ys) == rev_int ys @ rev_int xs)
-= admit()
+let rec snoc_append (xs ys : list int) (z : int)
+  : Lemma (snoc (xs @ ys) z = xs @ snoc ys z)
+  = match xs with
+    | [] -> ()
+    | _::xss -> snoc_append xss ys z
 
-let rev_rev (xs : list int)
+let rec rev_append_int (xs ys : list int)
+  : Lemma (rev_int (xs @ ys) == rev_int ys @ rev_int xs)
+= match xs with
+  | [] -> ()
+  | x::xs' -> (
+    //assert (rev_int ((x :: xs') @ ys) = rev_int (x :: (xs' @ ys)));
+    //assert (rev_int (x :: (xs' @ ys)) = snoc (rev_int (xs' @ ys)) x);
+    rev_append_int xs' ys;
+    //assert (snoc (rev_int (xs' @ ys)) x = snoc (rev_int ys @ rev_int xs') x);
+    snoc_append (rev_int ys) (rev_int xs') x
+    //assert (snoc (rev_int ys @ rev_int xs') x = rev_int ys @ snoc (rev_int xs') x);
+    //assert (rev_int ys @ snoc (rev_int xs') x = rev_int ys @ rev_int xs)
+  )
+
+let rec snoc_int (xs : list int) (y : int)
+  : Lemma (snoc xs y = xs @ [y])
+  = match xs with
+    | [] -> ()
+    | _::xss -> snoc_int xss y
+
+let rec rev_rev (xs : list int)
   : Lemma (rev_int (rev_int xs) == xs)
-= admit()
+= 
+  match xs with
+  | [] -> ()
+  | x::xss -> (
+    //assert (rev_int (rev_int xs) == rev_int (rev_int (x::xss)));
+    //assert (rev_int (rev_int (x::xss)) = rev_int (snoc (rev_int xss) x));
+    snoc_int (rev_int xss) x;
+    //assert (rev_int (snoc (rev_int xss) x) = rev_int (rev_int xss @ [x]));
+    rev_append_int (rev_int xss) [x];
+    //assert (rev_int (rev_int xss @ [x]) = rev_int [x] @ rev_int (rev_int xss));
+    //assert (rev_int [x] @ rev_int (rev_int xss) = [x] @ rev_int (rev_int xss));
+    rev_rev xss
+    //assert ([x] @ rev_int (rev_int xss) = [x] @ xss);
+    //assert ([x] @ xss = xs)
+  )
 
 let rev_injective (xs ys : list int)
   : Lemma (requires rev_int xs == rev_int ys) (ensures xs == ys)
-= admit()
+= rev_rev xs;
+  //assert (xs = rev_int (rev_int xs));
+  //assert (rev_int (rev_int xs) = rev_int (rev_int ys));
+  rev_rev ys
+  //assert (rev_int (rev_int ys) = ys)
